@prefix : <http://www.semanticweb.org/jioannou/ontologies/2017/2/actors-ttl#> .
@prefix owl: <http://www.w3.org/2002/07/owl#> .
@prefix rdf: <http://www.w3.org/1999/02/22-rdf-syntax-ns#> .
@prefix xml: <http://www.w3.org/XML/1998/namespace> .
@prefix xsd: <http://www.w3.org/2001/XMLSchema#> .
@prefix rdfs: <http://www.w3.org/2000/01/rdf-schema#> .
@prefix usdl-core: <http://www.linked-usdl.org/ns/usdl-core#> .

<http://www.semanticweb.org/jioannou/ontologies/2017/2/actors-ttl> a owl:Ontology ;
	rdfs:comment "The 'Actors' ontology describes the various business roles of an actor that may be part of the system ontology. This ontology extends the business role that is defined through the usdl-core ontology, and it is one of the two parts that will consist the Privacy Module topography."@en .
# 
# 
# #################################################################
# #
# #    Data properties
# #
# #################################################################
# 
# 
# http://www.semanticweb.org/jioannou/ontologies/2017/2/actors-ttl#ActorsProps

:ActorsProps a owl:DatatypeProperty ;
	rdfs:subPropertyOf owl:topDataProperty ;
	rdfs:comment "Represents the Actors data properties. Actor props are consisted by all the information that describe the existance and the purpose of each actor classification type."@en .
# 
# http://www.semanticweb.org/jioannou/ontologies/2017/2/actors-ttl#DataActions

:DataActions a owl:DatatypeProperty ;
	rdfs:subPropertyOf :ActorsProps ;
	rdfs:comment "Represents all actions that an actor can perform."@en .
# 
# http://www.semanticweb.org/jioannou/ontologies/2017/2/actors-ttl#Description

:Description a owl:DatatypeProperty ;
	rdfs:subPropertyOf :ActorsProps ;
	rdfs:comment "Represents a data property of the description that describes further an actor's purpose."@en .
# 
# http://www.semanticweb.org/jioannou/ontologies/2017/2/actors-ttl#Name

:Name a owl:DatatypeProperty ;
	rdfs:subPropertyOf :ActorsProps ;
	rdfs:comment "Represents a data property of the actor's full name."@en .
# 
# 
# 
# #################################################################
# #
# #    Classes
# #
# #################################################################
# 
# 
# http://www.linked-usdl.org/ns/usdl-core#BusinessRole

usdl-core:BusinessRole a owl:Class ;
	rdfs:comment "Represents the class of the 'Business Role'. The Business Roles describe the role that an entity may play within a service (e.g. Provider). One may define as many roles as necessary by defining subclasses of Business Role."@en ;
	rdfs:isDefinedBy <http://www.linked-usdl.org/ns/usdl-core> .
# 
# http://www.semanticweb.org/jioannou/ontologies/2017/2/actors-ttl#Actors

:Actors a owl:Class ;
	rdfs:subClassOf usdl-core:BusinessRole ;
	rdfs:comment "Represents the class of the 'Actors'. It is defined as a subclass of the core business role and describes the users that are defined in a privacy policy and have a direct or indirect interaction with the provided data"@en .
# 
# http://www.semanticweb.org/jioannou/ontologies/2017/2/actors-ttl#AuthorisedPerson

:AuthorisedPerson a owl:Class ;
	rdfs:subClassOf :Owners ;
	rdfs:comment "Represents the class of the 'Authorized Person'. The class is consisted by any authorized entity that is allowed to provide and manage the input raw data (public and sensitive information)."@en .
# 
# http://www.semanticweb.org/jioannou/ontologies/2017/2/actors-ttl#AuthorityRegulator

:AuthorityRegulator a owl:Class ;
	rdfs:subClassOf :Actors ;
	owl:disjointWith :Owners ;
	rdfs:comment "Represents the class of 'Authority/Regulator'. It is the entity that is responsible for the verification of the statutes and regulations that apply to the data processing by the various end users."@en .
# 
# http://www.semanticweb.org/jioannou/ontologies/2017/2/actors-ttl#Owners

:Owners a owl:Class ;
	rdfs:subClassOf :Actors ;
	owl:disjointWith :ThirdPartyUsers ;
	rdfs:comment "Represents the class of 'Owners'. These are the actors (Person of Interest or Authorized Person(s)) that are the 'original' data providers to the service (public and sensitive information) to the system."@en .
# 
# http://www.semanticweb.org/jioannou/ontologies/2017/2/actors-ttl#PersonOfInterest

:PersonOfInterest a owl:Class ;
	rdfs:subClassOf :Owners ;
	rdfs:comment "Represents the class of the 'Person of Interest'. The class is consisted by the entity that provides the input raw data (public and sensitive information)."@en .
# 
# http://www.semanticweb.org/jioannou/ontologies/2017/2/actors-ttl#SystemUsers

:SystemUsers a owl:Class ;
	rdfs:subClassOf :Actors ;
	rdfs:comment "Represents the class of 'System Users'. These are the entities that consist the service/system and their work is strictly related from it."@en .
# 
# http://www.semanticweb.org/jioannou/ontologies/2017/2/actors-ttl#ThirdPartyEndUsers

:ThirdPartyEndUsers a owl:Class ;
	rdfs:subClassOf :ThirdPartyUsers ;
	rdfs:comment "Represents the class of 'Third Party End Users'. Third-party end users do not belong in the organization and they utilize the information provided either by the initial service provider or from a third-party provider."@en .
# 
# http://www.semanticweb.org/jioannou/ontologies/2017/2/actors-ttl#ThirdPartyProviders

:ThirdPartyProviders a owl:Class ;
	rdfs:subClassOf :ThirdPartyUsers ;
	rdfs:comment "Represents the class of the 'Thrid Party Providers'. Third-party providers are considered: an end user that utilizes the data from the initial service provider based on the PLA and at the same time serves as an independent provider to other third-party end users giving access to the same (or modified) data."@en .
# 
# http://www.semanticweb.org/jioannou/ontologies/2017/2/actors-ttl#ThirdPartyUsers

:ThirdPartyUsers a owl:Class ;
	rdfs:subClassOf :Actors ;
	rdfs:comment "Represents the class of the 'Third Party Users'. The users that do not belong in the organization/system, where the Owners provide directly their information."@en .
# 
# Generated by the OWL API (version 4.2.6.20160910-2108) https://github.com/owlcs/owlapi
